Refactor vec_push

theories/typing/lib/vec/vec_pushpop.v
@@ -1,6 +1,6 @@
 From lrust.typing Require Export type.
-From lrust.typing Require Import array_util uniq_util typing lib.option.
-From lrust.typing.lib.vec Require Import vec.
+From lrust.typing Require Import array_util uniq_util typing.
+From lrust.typing.lib Require Import option vec_util vec.vec.
 Set Default Proof Using "Type".
 
 Open Scope nat.
@@ -12,110 +12,53 @@ Section vec_pushpop.
   Definition vec_push {𝔄} (ty: type 𝔄) : val :=
     fn: ["v"; "x"] :=
       let: "v'" := !"v" in delete [ #1; "v"];;
-      let: "len" := !("v'" +ₗ #1) in let: "ex" := !("v'" +ₗ #2) in
-      "v'" +ₗ #1 <- "len" + #1;;
-      withcont: "push":
-        if: "ex" ≤ #0 then
-          "v'" +ₗ #2 <- "len";; let: "l" := !"v'" in
-          let: "l'" := new [(#2 * "len" + #1) * #ty.(ty_size)] in
-          memcpy ["l'"; "len" * #ty.(ty_size); "l"];;
-          delete ["len" * #ty.(ty_size); "l"];;
-          "v'" <- "l'";; "push" []
-        else
-          "v'" +ₗ #2 <- "ex" - #1;; "push" []
-      cont: "push" [] :=
-        !"v'" +ₗ "len" * #ty.(ty_size) <-{ty.(ty_size)} !"x";;
-        delete [ #ty.(ty_size); "x"];;
-        let: "r" := new [ #0] in return: ["r"].
+      vec_push_core ty ["v'"; "x"];;
+      delete [ #ty.(ty_size); "x"];;
+      let: "r" := new [ #0] in return: ["r"].
 
   Lemma vec_push_type {𝔄} (ty: type 𝔄) :
     typed_val (vec_push ty) (fn<α>(∅; &uniq{α} (vec_ty ty), ty) → ())
       (λ post '-[(al, al'); a], al' = al ++ [a] → post ()).
   Proof.
     eapply type_fn; [apply _|]=> α ??[v[x[]]]. simpl_subst.
-    iIntros (tid (vπ & aπ &[]) ?) "#LFT #TIME #PROPH #UNIQ #E Na L C /=(v & x &_) #Obs".
+    iIntros (tid (vπ & bπ &[]) ?) "#LFT #TIME #PROPH #UNIQ #E Na L C /=(v & x &_) #Obs".
     rewrite !tctx_hasty_val. iDestruct "v" as ([|dv]) "[_ v]"=>//.
-    case v as [[|v|]|]=>//. iDestruct "v" as "[(%vl & >↦ & [#LftIn uniq]) †]".
+    case v as [[|v|]|]=>//. iDestruct "v" as "[(%vl & >↦v & [#LftIn uniq]) †v]".
     case vl as [|[[|v'|]|][]]; try by iDestruct "uniq" as ">[]".
-    iDestruct "x" as ([|dx]) "[⧖x x]"=>//. case x as [[|x|]|]=>//.
-    rewrite heap_mapsto_vec_singleton. wp_read. wp_let. wp_bind (delete _).
-    rewrite -heap_mapsto_vec_singleton freeable_sz_full.
-    iApply (wp_persistent_time_receipt with "TIME ⧖x"); [done|].
-    iApply (wp_delete with "[$↦ $†]"); [done|]. iIntros "!>_ ⧖x".
+    iDestruct "x" as ([|dx]) "[⧖x x]"=>//. case x as [[|x|]|]=>//=.
+    iDestruct "x" as "[↦ty †x]". rewrite heap_mapsto_vec_singleton. wp_read.
     iDestruct "uniq" as (du ξi [? Eq2]) "[Vo Bor]".
     move: Eq2. set ξ := PrVar _ ξi=> Eq2.
     iMod (lctx_lft_alive_tok α with "E L") as (?) "(α & L & ToL)"; [solve_typing..|].
     iMod (bor_acc with "LFT Bor α") as "[(%&%& ⧖u & Pc & ↦vec) ToBor]"; [done|].
     wp_seq. iDestruct (uniq_agree with "Vo Pc") as %[<-<-].
-    rewrite split_mt_vec. case du as [|du]=>//.
-    iDestruct "↦vec" as (? len ex aπl Eq1) "(↦ & ↦tys & (%wl &%& ↦ex) & †)".
-    rewrite !heap_mapsto_vec_cons shift_loc_assoc. iDestruct "↦" as "(↦₀ & ↦₁ & ↦₂ &_)".
-    do 2 (wp_op; wp_read; wp_let). do 2 wp_op. wp_write.
-    have ->: (len + 1)%Z = S len by lia.
-    iCombine "⧖u ⧖x" as "#⧖"=>/=. set d := du `max` dx.
+    rewrite split_mt_vec. case du as [|du]=>//=.
+    iDestruct "↦vec" as (? len ex aπl Eq1) "(↦l & ↦tys & ↦ex & †)".
+    wp_bind (delete _). rewrite -heap_mapsto_vec_singleton freeable_sz_full.
+    iApply (wp_persistent_time_receipt with "TIME ⧖x"); [done|].
+    iApply (wp_delete with "[$↦v $†v]"); [done|]. iIntros "!>_ ⧖x".
+    iCombine "⧖u ⧖x" as "#⧖". wp_seq. wp_bind (vec_push_core _ _).
+    iApply (wp_vec_push_core with "[↦l ↦tys ↦ex † ↦ty]"). { iExists _, _. iFrame. }
+    iIntros "!>(%&%& ↦ & ↦tys & ↦ex & † & (%& %Len & ↦x))". wp_seq.
+    rewrite freeable_sz_full. wp_bind (delete _).
+    iApply (wp_delete with "[$↦x †x]"); [lia|by rewrite Len|]. iIntros "!>_".
+    wp_seq. set vπ' := λ π, (lapply (vsnoc aπl bπ) π, π ξ).
     iMod (uniq_update with "UNIQ Vo Pc") as "[Vo Pc]"; [done|].
-    set push := (rec: "push" _ := _)%E.
-    iAssert (
-      (∃(l: loc) (ex: nat), v' ↦∗ [ #l; #(S len); #ex] ∗
-        ([∗ list] i ↦ aπ ∈ aπl, (l +ₗ[ty] i) ↦∗: ty.(ty_own) aπ du tid) ∗
-        (l +ₗ[ty] len) ↦∗len (S ex * ty.(ty_size)) ∗
-        freeable_sz' ((S len + ex) * ty.(ty_size)) l) -∗
-      WP push [] {{ _, cont_postcondition }})%I
-      with "[L ToL Na C Vo Pc ToBor x]" as "push".
-    { iIntros "/=(%&%& ↦ & ↦tys & (%vl & %Len & ↦ex) & †)".
-      rewrite !heap_mapsto_vec_cons. iDestruct "↦" as "(↦₀ & ↦₁ & ↦₂ &_)".
-      rewrite /push. wp_rec. wp_read. do 2 wp_op. wp_bind (_ <-{_} !_)%E.
-      move: {Len}(app_length_ex vl _ _ Len)=> [vl'[?[->[Len ?]]]].
-      rewrite heap_mapsto_vec_app shift_loc_assoc_nat Len -Nat2Z.inj_mul.
-      iDestruct "↦ex" as "[↦ ↦ex]". iDestruct "x" as "[(%& ↦x & ty) †x]".
-      iDestruct (ty_size_eq with "ty") as %Sz. rewrite freeable_sz_full.
-      iApply (wp_memcpy with "[$↦ $↦x]"); [lia..|]. iIntros "!> [↦ ↦x]". wp_seq.
-      wp_bind (delete _). iApply (wp_delete with "[$↦x †x]"); [lia|by rewrite Sz|].
-      iIntros "!>_". wp_seq. set vπ' := λ π, (lapply (vsnoc aπl aπ) π, π ξ).
-      iMod ("ToBor" with "[↦₀ ↦₁ ↦₂ ↦tys ↦ ty ↦ex † Pc]") as "[Bor α]".
-      { iNext. iExists _, _. rewrite split_mt_vec. iFrame "⧖ Pc".
-        iExists _, _, _, (vsnoc aπl _).
-        rewrite !heap_mapsto_vec_cons heap_mapsto_vec_nil shift_loc_assoc.
-        iFrame "↦₀ ↦₁ ↦₂ †". iSplit; [done|]. iSplitR "↦ex"; last first.
-        { iExists _. rewrite/= plus_comm. by iFrame. }
-        iNext. rewrite vec_to_list_snoc big_sepL_app. iSplitL "↦tys".
-        { iClear "#". iStopProof. do 6 f_equiv. apply ty_own_depth_mono. lia. }
-        rewrite/= right_id. iExists _. rewrite vec_to_list_length Nat.add_0_r.
-        iFrame "↦". iApply ty_own_depth_mono; [|done]. lia. }
-      iMod ("ToL" with "α L") as "L".
-      iApply (type_type +[#v' ◁ &uniq{α} (vec_ty ty)] -[vπ']
-        with "[] LFT TIME PROPH UNIQ E Na L C [-] []").
-      - iApply type_new; [done|]. intro_subst.
-        iApply type_jump; [solve_typing|solve_extract|solve_typing].
-      - rewrite/= right_id (tctx_hasty_val #_). iExists _.
-        iFrame "⧖ LftIn". iExists _, _. rewrite /uniq_body.
-        rewrite (proof_irrel (@prval_to_inh (listₛ 𝔄) (fst ∘ vπ'))
-          (@prval_to_inh (listₛ 𝔄) (fst ∘ vπ))). by iFrame.
-      - iApply proph_obs_impl; [|done]=> π.
-        move: (equal_f Eq1 π) (equal_f Eq2 π)=>/=. case (vπ π)=>/= ??->-> Imp Eq.
-        apply Imp. move: Eq. by rewrite vec_to_list_snoc lapply_app. }
-    rewrite /push. wp_let. wp_op. wp_case. case ex as [|ex']=>/=; last first.
-    { do 2 wp_op. have ->: (S ex' - 1)%Z = ex' by lia. wp_write.
-      iApply "push". iExists _, _.
-      rewrite !heap_mapsto_vec_cons heap_mapsto_vec_nil shift_loc_assoc.
-      iFrame "↦tys ↦₀ ↦₁ ↦₂". iSplitL "↦ex". { iExists _. iFrame. iPureIntro. lia. }
-      iClear "#". iStopProof. f_equiv. lia. }
-    wp_op. wp_write. wp_read. wp_let. do 3 wp_op. wp_bind (new _).
-    iApply wp_new; [lia|done|]. iIntros "!>" (?) "[†' ↦']". wp_let. wp_op.
-    have ->: ∀sz: nat, ((2 * len + 1) * sz)%Z = (len + S len) * sz by lia.
-    rewrite trans_big_sepL_mt_ty_own plus_0_r Nat2Z.id Nat.mul_add_distr_r
-      repeat_app heap_mapsto_vec_app.
-    iDestruct "↦tys" as (?) "[↦ tys]". iDestruct "↦'" as "[↦' ↦ex']".
-    iDestruct (big_sepL_ty_own_length with "tys") as %Len. wp_bind (memcpy _).
-    iApply (wp_memcpy with "[$↦' $↦]"); [rewrite repeat_length; lia|lia|].
-    iIntros "!>[↦' ↦]". wp_seq. wp_op. rewrite -Nat2Z.inj_mul. wp_bind (delete _).
-    iApply (wp_delete with "[$↦ †]"); [lia|by rewrite Len|]. iIntros "!>_".
-    wp_seq. wp_write. iApply "push". iExists _, _.
-    rewrite !heap_mapsto_vec_cons heap_mapsto_vec_nil shift_loc_assoc.
-    iFrame "↦₀ ↦₁ ↦₂". iSplitL "↦' tys".
-    { rewrite trans_big_sepL_mt_ty_own. iExists _. iFrame. } iSplitR "†'".
-    - iExists _. rewrite repeat_length. iFrame "↦ex'". by rewrite repeat_length.
-    - by have <-: ∀sz, sz + (len + len) * sz = len * sz + (sz + len * sz) by lia.
+    iMod ("ToBor" with "[↦ ↦tys ↦ex † Pc]") as "[Bor α]".
+    { iNext. iExists _, _. rewrite split_mt_vec. iFrame "⧖ Pc".
+      iExists _, _, _, (vsnoc _ _). by iFrame. }
+    iMod ("ToL" with "α L") as "L".
+    iApply (type_type +[#v' ◁ &uniq{α} (vec_ty ty)] -[vπ']
+      with "[] LFT TIME PROPH UNIQ E Na L C [-] []").
+    - iApply type_new; [done|]. intro_subst.
+      iApply type_jump; [solve_typing|solve_extract|solve_typing].
+    - rewrite/= right_id (tctx_hasty_val #_). iExists _.
+      iFrame "⧖ LftIn". iExists _, _. rewrite /uniq_body.
+      rewrite (proof_irrel (@prval_to_inh (listₛ 𝔄) (fst ∘ vπ'))
+        (@prval_to_inh (listₛ 𝔄) (fst ∘ vπ))). by iFrame.
+    - iApply proph_obs_impl; [|done]=> π.
+      move: (equal_f Eq1 π) (equal_f Eq2 π)=>/=. case (vπ π)=>/= ??->-> Imp Eq.
+      apply Imp. move: Eq. by rewrite vec_to_list_snoc lapply_app.
   Qed.
 
   Definition vec_pop {𝔄} (ty: type 𝔄) : val :=
